%! Author = joshu
%! Date = 9/14/20

% Preamble
\documentclass[11pt]{article}

% Packages
\usepackage{amsmath}
\renewcommand{\thesubsection}{\thesection.\alph{subsection}}
\newcommand{\bv}[2]{\big\vert_{#1}^{#2}}
\usepackage{hyperref}
\usepackage{amssymb}
% Document
\begin{document}
    \section[Question 1]{$\int\frac{x+1}{x^2+2x-3}$}
    \label{sec:1}
    \subsection[1.a]{Solve integral with partial Fraction}
    \label{subsec:1a}
    \begin{flalign*}
        \int\frac{x+1}{(x-2)(x-1)}dx && \\
        \int\frac{A}{x-2} + \frac{B}{x-1}dx &= \frac{x+1}{\mathellipsis} \\
        \\
        A(x-1) + B(x-2) &= x + 1 && \\
        -1B &= 2 && x = 1 && && && \\
        B &= -2 && \\
        A &= 3 && x = 2 \\
        \int\frac{3}{x-2} - \frac{2}{x-1}dx \\
        \\
        3\ln(|x-2|) - \ln(|x-1|) + c \\
    \end{flalign*}
    \subsection[1.b]{Solve using another Technique}
    \label{subsec:1b}
    \begin{flalign*}
        \int\frac{x+1}{x^2{+2x-3}} && u = x^2 + 2x -3 &&\\
        && du = 2x + 2 \\
        \frac{1}{2}\int\frac{du}{u}&& \frac{1}{2}du = x + 1 \\
        \frac{1}{2}\ln(|u|) + c \\
        \frac{1}{2}\ln(|x^2 + 2x - 3)
    \end{flalign*}
    \subsection[1.c]{Evaluate $\int_{0}^{5}dx$ or show that it diverges}
    \label{subsec:1c}
    \begin{flalign*}
        \int_{0}^{5}\frac{x+1}{x^2{+2x-3}} && x \neq 1 && && \\
        \lim_{a\to1}\int_{0}^{a}\frac{x+1}{x^2+2x-3} + \lim_{b\to5}\int_{1}^{b}\frac{x+1}{x^2+2x-3} && u = x^2 + 2x -3\\
        \lim_{a\to1}\frac{1}{2}\int\frac{du}{u} + \frac{1}{2}\lim_{b\to5}\int\frac{du}{u} && \frac{1}{2}du = x + 1 \\
        \frac{1}{2}\ln(|u|) +  \frac{1}{2}\ln(|u|) \\
        \lim_{a\to1}\ln(\sqrt{x^2+2x-3}) \bv{0}{a} + \mathellipsis \\
        \ln(\sqrt{1^2 + 2 - 3}) \\
        \ln(0) \to DNE \therefore\ Diverges
    \end{flalign*}
    \section[Question 2]{Find using given values}
    \label{sec:2}
    \subsection[2.a]{$\int_{0}^{2} 3(f(x)-2)dx$}
    \label{subsec:2a}
    \begin{flalign*}
        3 \int_{0}^{2} f(x)dx - 3 \int_{0}^{2} 2dx && \\
        3(\frac{1}{2}*6) - 3 (2x \bv{0}{2}) &&\int_{0}^{2} f(x) = \frac{1}{2} \int_{-2}^{2} f(x)dx &&\\
        9 - 3 (2(2) - 0) \\
        9 - 3(4) = -3
    \end{flalign*}
    \subsection[2.b]{$ \int_{-2}^{-1} f(x)dx$}
    \label{subsec:2b}
    \begin{flalign*}
        \int_{-2}^{0}f(x) = 3 \\
        \int_{0}^{1}f(x) = \int_{-1}^{0} f(x) = 1  \\
        \int_{-2}^{0}f(x) + \int_{-1}^{0}f(x) = \int_{-2}^{-1} f(x) \\
        3 + 1 = \int_{-2}^{-1} f(x) \\
        \int_{-2}^{-1} f(x) = 4
    \end{flalign*}
    \subsection[2.c]{$ \int_{-1}^{2} xf(x)$}
    \label{subsec:2c}
    \begin{flalign*}
        \int_{0}^{1} xf(x)dx = \int_{-1}^{0} xf(x)dx = \frac{1}{2} \\
        \int_{-1}^{2} xf(x) &= \int_{-1}^{0} + \int_{0}^{2} xf(x)dx \\
        &= \frac{1}{2} + 4 \\
        &= \frac{9}{2}
    \end{flalign*}
    \section[Question 3]{f(x) and f'(x) are continuous. Use the table}
    \label{sec:3}
    \subsection[3.a]{$\int_{0}^{1} f'(x)$}
    \label{subsec:3a}
    \begin{flalign*}
        f(x) \bv{0}{1} &&\\
        f(1) - f(0) \\
        5 - 3 = 2
    \end{flalign*}
    \subsection[3.b]{$\int_{0}^{2} (f'(x)\sin(x) + f(x)\cos(x))$}
    \label{subsec:3b}
    \begin{flalign*}
        \int_{0}^{2} f'(x)sin(x)dx && u = \sin(x)\ && dv = f'(x) \\
        && du = cos(x)\ && v = f(x) \\
        f(x)\sin(x)\bv{0}{2} - \int_{0}^{2} f(x)cos(x)dx \\
        f(2)sin(2) - f(0)sin(0) - \int_{0}^{2} f(x)cos(x)dx \\
        8\sin(2) - \int_{0}^{2} f(x)cos(x)\\
        \\
        \int_{0}^{2} f(x)cos(x)dx   && u = f(x) && dv = cos(x) \\
        -\sin(x)f(x)\bv{0}{2} - \int_{0}^{2} sin(x)f'(x)dx && du = f'(x) && v = -\sin(x) \\
        -\sin(2)f(2) + sin(0)f(0) +\int_{0}^{2} sin(x)f'(x)dx\\
        -8\sin(2) + \int_{0}^{2} sin(x)f'(x)dx\\
        \\
        \int_{0}^{2} f'(x)sin(x)dx = 8sin(2) - \int_{0}^{2} f(x)cos(x) \\
        \int_{0}^{2} f'(x)sin(x)dx = 8sin(2) - (-8\sin(2) + \int_{0}^{2} sin(x)f'(x)dx)\\
        \text{Which just simplifies to 0 ... dang}
    \end{flalign*}
    \subsection[3.c]{$ \int_{0}^{3} \frac{f'(x)e^x - f(x)e^x}{(e^x)^2}dx$}
    \label{subsec:3c}
    \begin{flalign*}
        && u = f(x)e^x \\
        && du = f(x)e^x + e^{x}f'(x) \\
        && du = e^x(f(x) + f'(x)) \\
        \int_{0}^{3} \frac{f'(x)}{e^x} - \int_{0}^{3} \frac{f(x)}{e^x}
    \end{flalign*}
    \subsection[3.d]{$ \int_{0}^{1} f(x)f'(x)$}
    \label{subsec:3d}
    \begin{flalign*}
        \int udu&& u &= f(x) &&\\
        \int_{3}^{5}udu && du &= f'(x) &&\\
        \frac{1}{2}u^{2} \bv{3}{5} \\
        \frac{1}{2}(5)^2 - \frac{1}{2}3^3 \\
        \frac{25}{2} - \frac{9}{2} = 8
    \end{flalign*}
    \section[Question 4]{Average value = $ \frac{1}{b-a}\int_{a}^{b} f(x)dx$}
    \label{sec:4}
    \subsection[4.a]{Find number(s) b, so a.v of $f(x) = 2 + 6x -3x^2$ on interval [0,b] equal to 3}
    \label{subsec:4a}
    \begin{flalign*}
        \frac{1}{b-0} \int_{0}^{b} 2 + 6x -3x^2 dx = 3 \\
        \frac{1}{b}( 2x + 3x^2 - x^3 )\bv{0}{b} = 3 \\
        \frac{1}{b}(2b + 3b^2 - b^3 - 0) = 3 \\
        2 + 3b - b^2 = 3 \\
        -1 + 3b - b^2 = 0 \\
        -(b^2 - 3b + 1) = 0
    \end{flalign*}
    \subsection[\textbf{4}]{}
    \label{subsec:4b}
    \begin{flalign*}
        \frac{4+5}{2} = \frac{9}{2}
    \end{flalign*}
    \section[Question 5]{}
    \label{sec:5}
    \subsection[5.a]{$\int_{1}^{\infty} \frac{1}{(x+1)(2x+3)}dx$}
    \label{subsec:5a}
    \begin{flalign*}
        \lim_{a\to\infty}\int_{1}^{a} \frac{1}{(x+1)(2x+3)}dx\\
        \frac{A}{x+1} + \frac{B}{2x +3} \\
        A(2x+3) + B(x+1) = 1 \\
        A(1) = 1&& x = -1 &&\\
        B(-\frac{3}{2} + 1) = 1 && x = \frac{-3}{2}\\
        -\frac{1}{2}B = 1 \\
        B = -2 \\
        \lim_{a\to\infty}\int_{1}^{a}\frac{1}{x+1}  - \lim_{a\to\infty} 2\int_{1}^{a}  \frac{1}{2x+3} \\
        \lim_{a\to\infty}\ln(|x+1|)\bv{1}{a} - 2\lim_{a\to\infty}\ln(|2x+3|) * \frac{1}{2} \\
        \lim_{a\to\infty}\ln(|x+1|)\bv{1}{a} - \lim_{a\to\infty}\ln(|2x+3|) \\
        \lim_{a\to\infty} \ln\frac{|x+1|}{|2x+3|}\bv{1}{a} \\
        LH \to \lim_{a\to\infty}\ln\frac{a+1}{2a+3} - \ln\frac{2}{5} \\
        \lim_{a\to\infty}\ln(\frac{1}{2}) + \ln(\frac{5}{2}) \\
        \ln(\frac{5}{4}) \\
    \end{flalign*}
    \subsection[5.b]{$ \int_{0}^{e} \ln(x)dx$}
    \label{subsec:5b}
    \begin{flalign*}
        \lim_{a\to0}\int_{a}^{e} \ln(x) \\
        u = ln(x) && dv = 1 && && \\
        du = \frac{1}{x} && v = x && && \\
        \lim_{a\to0}xln(x) \bv{a}{e} - \lim_{a\to0}\int_{a}^{e} 1 dx \\
        \lim_{a\to0}\frac{ln(x)}{\frac{1}{x}}\bv{a}{e} -  \lim_{a\to0}x\bv{a}{e} \\
        LH \frac{1}{1/e} - \frac{\ln(a)}{1/a} - e \\
        e -  \frac{1/a}{-1/a^2} - e \\
        \lim_{a\to0}\frac{a^{-1}}{-a^{-2}}
    \end{flalign*}
    \subsection[5.c]{$ \int_{-\pi/2}^{\pi/2} \frac{x\cos(x^2)}{(\sin(x^2))^2}$}
    \label{subsec:5c}
    \begin{flalign*}
        \lim_{a\to0}\int_{-\pi/2}^{a}\frac{x\cos(x^2)}{(\sin(x^2))^2} + \lim_{b\to0}\int_{b}^{\pi/2}\frac{x\cos(x^2)}{(\sin(x^2))^2} \\
        \lim_{b\to0}\frac{1}{2}\int_{b}^{\pi/2}\frac{du}{u^2} && u &= sin(x^2)  &&\\
        \lim_{b\to0}\frac{1}{2}\int_{b}^{\pi/2}u^{-2} && du &= 2xcos(x^2) &&\\
        \frac{1}{2}\lim_{b\to0}(- u^{-1}) \bv{b}{\pi/2}&& \frac{1}{2}du &= xcos(x^2) &&\\
        \frac{1}{2}\lim_{b\to0}(-\frac{1}{\sin(x^2)})\bv{b}{\pi/2}
    \end{flalign*}

\end{document}