%! Author = joshu
%! Date = 9/10/20

% Preamble
\documentclass[11pt]{article}
\newcommand{\bv}[2]{\big\vert_{#1}^{#2}}
\title{Integration Practice}
\author{Colinn Kaeo, Connor Shovlin, Denali Termin, Joshua Petitma}
% Packages
\usepackage{amsmath}
\usepackage{amssymb}

% Document
\begin{document}
    \maketitle
    \begin{enumerate}
        \item $\int xe^x$
        \begin{align*}
            xe^x - \int e^x + c&& u = x && dv = e^x \\
            xe^x - e^x dx + c&& du = 1 && v = e^x \\
        \end{align*}
        \item $\int xe^{x^2}$
        \begin{align*}
            \frac{1}{2}\int e^u du&& u = x^2 \\
            \frac{1}{2} e^u + c && du = 2x \\
            \frac{1}{2}e^{x^2} + c&& \frac{1}{2}du = x
        \end{align*}
        \item $\int \frac{x}{\sqrt{1-x^4}}$
        \begin{align*}
            \int \frac{x}{\sqrt{1 - (x^2)^{2}}}dx \\
            \frac{1}{2}\arcsin(x^2) + c
        \end{align*}
        \item $\int 2x\ln(x)dx$
        \begin{align*}
            \label{q:5}
            x^2 \ln(x) - \int x^2 * \frac{1}{x}dx && u = \ln(x) && dv = 2x \\
            x^2 \ln(x) - \int xdx && du = \frac{1}{x} && v = x^2 \\
            x^2 \ln(x) - \frac{x^2}{2} + c
        \end{align*}
        \item $\int \frac{x + 7}{\sqrt{5-x}}$
        \begin{align*}
            \int \frac{12-u}{\sqrt{u}}&& u &= 5 - x \\
            12\int \frac{1}{\sqrt{u}} - \int \frac{u}{\sqrt{u}}&& 5 - u &= x \\
            12 * -2\sqrt{u} - \int \sqrt{u}&& 12 - u &= x+7 \\
            - 24\sqrt{u} - \frac{2}{3}u^{3/2}&& -du &= 1 \\
            - 24\sqrt{5-x} - \frac{2}{3}(5-x)^{3/2} + c
        \end{align*}
        \item $\arcsin x$
        \begin{align*}
            \label{q:6}
            u = \arcsin(x) && dv = 1 \\
            du = \frac{1}{\sqrt{1 - x^2}} && v = x \\
            x\arcsin(x) - \int \frac{x}{\sqrt{1 - x^2}} \\
            x\arcsin(x) + \frac{1}{2}\int\frac{1}{\sqrt{u}}du && u &= 1 - x^2 \\
            x\arcsin(x) + \sqrt{u} + c&& du &= -2x \\
            arcsin(x) + \sqrt{1-x^2} + c&& -\frac{1}{2}du &= x
        \end{align*}
        \item $\int x^5\sqrt{x^3 +1}$
        \begin{align*}
            \label{q:7}
            \int x^3 * x^2\sqrt{x^3 + 1}&& u = x^3 + 1 \\
            \frac{1}{3}\int (u - 1)\sqrt{u}&& u - 1 = x^3 \\
            \frac{1}{3} \int u^{3/2} - u^{1/2}&& du = 3x^2 \\
            \frac{1}{3} * (\frac{2}{5} u^{5/2} - \frac{2}{3}u^{3/2}) \\
            \frac{2}{15}(x^3 + a)^{5/2} - \frac{2}{9}(x^3 + 1)^{3/2} + c
        \end{align*}
        \item $\int \frac{1}{x^2 + 6x + 8}$
        \begin{align*}
            \label{q:8}
            \frac{1}{(x+4)(x+2)} \\
            \frac{A}{x+4} + \frac{B}{x+2} = \frac{1}{...} \\
            A(x+2) + B(x+4) = 1  \\
            B(-2 +4) = 1 && x = -2 \\
            B = \frac{1}{2} \\
            A (-4 + 2)  = 1 && x = -4 \\
            A = -\frac{1}{2} \\
            \frac{1}{2} \int -\frac{1}{x+4} + \frac{1}{x+2} \\
            \frac{1}{2} (- \ln(x+4) + ln(x+2)) + c
        \end{align*}
    \end{enumerate}
    \begin{enumerate}
        \item $\int_{-3}^{1} \frac{1}{x^2 -x -2}dx$
        \begin{align*}
            \label{q2:1}
            \int_{-3}^{1} \frac{1}{(x-2)(x+1)} \\
            \\
            \frac{A}{(x-2)} + \frac{B}{x+1} = \frac{1}{...}\\
            A (x+1) + B (x-2) \\
            B(-1 -2) &= 1 && x = -1 \\
            B &= -\frac{1}{3} \\
            A (2 + 1) &= 1 && x = 2 \\
            A &= \frac{1}{3} \\
            \frac{1}{3}\int_{-3}^{1}  \frac{1}{x-2} - \frac{1}{x+1} \\
            \frac{1}{3} (\int_{-3}^{-1} \frac{1}{x-2} - \frac{1}{x+1}dx + \int_{-1}^{1} \frac{1}{x-2} - \frac{1}{x+1})\\
            \frac{1}{3}(\ln(x-2) - ln(x+1))\bv{-3}{-1}  \\
            \frac{1}{3}(\ln(\frac{x-2}{x+1}) \bv{-3}{-1}) \\
            ln(\frac{-3}{0})  \to undefined \therefore Divergent\\
        \end{align*}
        \item $\int_{-\infty}^{\infty}\frac{1}{25 + x^2} $
        \begin{align*}
            \label{q2:2}
            \\
            \int_{0}^{\infty} \frac{1}{25 + x^2} && \int_{-\infty}^{0} \frac{1}{25 + x^2} \\
            \lim_{b\to\infty} \int_{0}^{b} \frac{1}{25 + x^2} && \lim_{a\to-\infty} \int_{a}^{0} \frac{1}{25 + x^2} \\
            \lim_{b\to\infty} \int_{0}^{b} \frac{1}{25 (1 + \frac{x^2}{25})} && \lim_{a\to-\infty} \int_{a}^{0} \frac{1}{25 (1 + \frac{x^2}{25})} \\
            \lim_{b\to\infty} \frac{1}{25}\int_{0}^{b} \frac{1}{(1 + \frac{x^2}{25})} && \lim_{a\to-\infty} \frac{1}{25}\int_{a}^{0} \frac{1}{(1 + \frac{x^2}{25})} \\
            \lim_{b\to\infty}\frac{1}{25}\arctan(\frac{x}{5}) * \frac{1}{5} \bv{0}{b}&& \lim_{a\to-\infty}\frac{1}{25}\arctan(\frac{x}{5}) * \frac{1}{5} \bv{a}{0}\\
            \lim_{b\to\infty} \frac{\arctan(x/5)}{25} \bv{0}{b} && \lim_{a\to-\infty} \frac{\arctan(x/5)}{25} \bv{a}{0} \\
            \lim_{b\to\infty} \frac{\arctan(b)}{25} + \frac{\arctan(0)}{25} && \frac{\arctan(0)}{25} + \lim_{a\to-\infty} \frac{\arctan(a)}{25} \\
            \frac{\pi/2}{25} && -\frac{\pi/2}{25} \\
            \\
            \frac{\pi/2}{25} -\frac{\pi/2}{25} &= 0 \therefore Convergent\\
        \end{align*}
        \item $\int_{5}^{\infty}\frac{1}{x^2 + x}dx $
        \begin{align*}
            \label{q2:3}
            \lim_{a\to\infty}\int_{5}^{a} \frac{1}{x(x+1)}dx \\
            \\
            \frac{A}{x} + \frac{B}{x+1} = \frac{1}{...}\\
            A(x+1) + B(x) &= 1 \\
            B(-1) &= 1 && x = -1 \\
            B &= -1 \\
            A &= 1 && x = 0 \\
            \lim_{a\to\infty} \int_{5}^{a} \frac{1}{x} - \frac{1}{x+1} \\
            \lim_{a\to\infty}\ln(x) - ln(x+1)\bv{5}{a} \\
            \lim_{a\to \infty}\ln\frac{x}{x+1}\bv{5}{a} \\
            L.H \to \lim_{a\to \infty}\ln\frac{a}{a+1} - \ln(\frac{5}{6}) \\
            \ln(1) - \ln(\frac{5}{6}) \\
            ln(\frac{6}{5})
        \end{align*}
        \item $ \int_{0}^{\pi}\tan(x)$
        \begin{align*}
            \label{q2:4}
            \int_{0}^{\pi} \frac{\sin x}{\cos x} && x \neq \frac{\pi}{2}\\
            \lim_{a\to \pi/2}\int_{0}^{a} \frac{\sin x}{\cos x} && \lim_{b\to \pi/2}\int_{b}^{\pi} \frac{\sin x}{\cos x}\\
           \lim_{a\to \pi/2}-\ln(|\cos x|) \bv{0}{a} &&\lim_{b\to \pi/2}-\ln(|\cos x|) \bv{b}{\pi} \\
            \lim_{a\to \pi/2} -\ln(\cos(a)) + \ln(cos(0)) && \lim_{b\to \pi/2} -\ln(|\cos(\pi)|) + \ln(|cos(b)|)\\
            -ln(0) + 0 && -ln(1) + ln(0)\\
            \ln(0) \to -\infty \therefore Divergent
        \end{align*}
        \item $ \int_{0}^{10}x^3\ln(x)$
        \begin{align*}
            \label{q2:5}
            \frac{x^4}{4}\ln(x)\bv{0}{10} - \int_{0}^{10}\frac{x^3}{4}dx && u = \ln(x) && dv = x^3 \\
            && du = \frac{1}{x} && v = \frac{x^4}{4} \\
            \frac{10^4}{4}ln(10) - \frac{x^4}{16}\bv{0}{10} \\
            \frac{10^4}{4}ln(10) - \frac{10^4}{16} &&  \therefore Convergent
        \end{align*}
    \end{enumerate}
\end{document}